%なんか日本語でコメントしとかないとvimが文字コード間違える
\documentclass[11pt]{jsarticle}
\usepackage{amssymb}
\usepackage{amsmath}
\usepackage{newtxmath}
\usepackage{newtxtext}
\usepackage[utf8]{inputenc}
\usepackage{bm}

\title{Error Terms for Logarithmic Hamiltonian}
\author{似鳥啓吾}

\begin{document}
\maketitle

A time transformed logarithmic Hamiltonian is
\begin{equation}
\Gamma = \ln (p_0 + T) - \ln U,
\end{equation}
where $T$ is kinetic energy, $U$ a negative potential,
$p_0$ a time momentum of which value is negative of
total energy $p_0 = -(T - U)$.
$\mathcal H = \mathcal T + \mathcal V$
Partial derivatives are
\begin{subequations}
\begin{align}
\frac{\partial}{\partial p_0} \Gamma =& \frac{1}{p_0 + T}, \\
\frac{\partial}{\partial p_i} \Gamma =& \frac{1}{p_0 + T} v_i, \\ %\frac{p_i}{m_i} \\
\frac{\partial}{\partial q_0} \Gamma =& 0, \\
\frac{\partial}{\partial p_i} \Gamma =& -\frac{1}{U} f_i,
\end{align}
\end{subequations}
with $v_i$ is velocity $v_i$ = $p_i / m_i = \partial T / \partial p_i$
and $f_i$ force $f_i = \partial U / \partial q_i$.

A Poisson bracket is
\begin{equation}
\{ A,\, B \} = \sum_{i=0}^N
\left(
\frac{\partial A}{\partial q_i}
\frac{\partial B}{\partial p_i}
-
\frac{\partial B}{\partial q_i}
\frac{\partial A}{\partial p_i}
\right).
\end{equation}

Now let us investigate
\begin{equation}
\begin{aligned}
\bigl\{ \ln (p_0 + T),\, -\ln U \bigr\} 
=& \sum_{i=1}^N
\frac{\partial}{\partial p_i} \left( \ln (p_0 + T) \right)
\frac{\partial}{\partial q_i} \left( \ln U \right) \\
=& \sum_{i=1}^N
\frac{1}{p_0 + T}\frac{1}{U} \bigl( v_i \cdot f_i \bigr).
\end{aligned}
\end{equation}
For $\partial / \partial q_0 = 0$, thus $i=0$ is not included in the summation range.
Now,
\begin{align}
\frac{\partial}{\partial p_i} \left\{ \ln (p_0 + T),\, -\ln U \right\} 
=&
\frac{1}{p_0 + T}\frac{1}{U}
\left[
	\frac{f_i}{m_i} - \frac{\sum_j \left( v_j \cdot f_j \right)}{p_0 + T} v_i  
\right],
\\
\frac{\partial}{\partial q_i} \left\{ \ln (p_0 + T),\, -\ln U \right\} 
=&
\frac{1}{p_0 + T}\frac{1}{U}
\left[
	\left( \sum_j \frac{\partial f_j}{\partial q_i} \cdot v_j \right)
	- \frac{\sum_j \left( v_j \cdot f_j \right)}{U} f_j
\right],
\end{align}
and
\begin{align}
\Bigl\{ \bigl\{ \ln (p_0 + T),\, -\ln U \bigr\},\, -\ln U \Bigr\}
=& 
	\sum_i \frac{\partial}{\partial p_i} \bigl\{ \ln (p_0 + T),\, -\ln U \bigr\}
	\cdot \frac{\partial}{\partial q_i} \ln U \nonumber \\
=&
	\frac{1}{p_0 + T}\frac{1}{U^2}
	\left[
		\sum_i \frac{{f_i}^2}{m_i} - \frac{{\left[\sum_j \left( v_j \cdot f_j \right)\right]}^2}{p_0 + T}
	\right],
\end{align}
\begin{align}
\Bigl\{ \bigl\{ -\ln U,\, \ln (p_0 + T) \bigr\},\, -\ln (p_0 + T) \Bigr\}
=& 
	-\sum_i \frac{\partial}{\partial q_i} \bigl\{ \ln (p_0 + T),\, -\ln U \bigr\}
	\cdot \frac{\partial}{\partial p_i} \ln (p_0 + T) \nonumber \\
=&
-\frac{1}{{(p_0 + T)}^2}\frac{1}{U}
	\left[
		\left( \sum_{i,j} \frac{\partial f_j}{\partial q_i} \cdot v_j \cdot v_i \right)
	-\frac{{\left[\sum_j \left( v_j \cdot f_j \right)\right]}^2}{U}
	\right].
\end{align}

Consider a Kepler problem
\[
U = p_0 + T = \frac{\mu}{r},\quad m_i=1, \quad f_i = - \frac{\mu r_i}{r^3}, \quad 
\frac{\partial f_i}{\partial q_j} = -\mu \left( \frac{\delta_{ij}}{r^3} - \frac{3 r_i r_j}{r^5} \right).
\]
Then,
\begin{align}
\{\{\mathcal T,\, \mathcal V \},\, \mathcal V\}
	= \frac{1}{\mu^2} \left[ \frac{\mu}{r} - {\left(\frac{\bm r \cdot \bm v}{r} \right)}^2 \right], \\
\{\{\mathcal V,\, \mathcal T \},\, \mathcal T\}
	= \frac{1}{\mu^2} \left[ v^2 - 2{\left(\frac{\bm r \cdot \bm v}{r} \right)}^2 \right].
\end{align}
Thus,
\begin{equation}
\{\{\mathcal T,\, \mathcal V \},\, \mathcal V\}
- \frac12
\{\{\mathcal V,\, \mathcal T \},\, \mathcal T\}
=
-\frac{1}{\mu^2}
\left[
	\frac12 v^2 - \frac{\mu}{r}
\right]
= \frac{p_0}{\mu^2},
\end{equation}
is proportional to the leading error term of the DKD mode.

%\begin{equation}
%\end{equation}

\end{document}
